attempts at reverse reverse

SomeMath/LearningRecursion.lean
@@ -7,3 +7,75 @@ universe u
 inductive List (α : Type u) where
   | empty : List α
   | cons : α → List α → List α
+
+
+open List
+
+def reverse {α : Type u} (as : List α) : List α :=
+  loop as empty
+where
+  loop : List α → List α → List α
+  | empty, ras => ras
+  | cons a ast, ras => loop ast (cons a ras)
+
+def len {α : Type u} : List α → Nat
+  | empty => 0
+  | cons _ as => 1 + (len as)
+
+theorem reverse_maintains_length {α : Type u} (as : List α)
+  : len as = len (reverse as) :=
+  List.recOn (motive := fun as => len as = len (reverse as))
+    as
+    (show len empty = len (reverse empty) from rfl)
+    (fun (a : α) (as : List α) (ih : len as = len (reverse as)) =>
+     show len (cons a as) = len (reverse (cons a as)) from
+     calc len (cons a as)
+      _ = 1 + len as := rfl
+      _ = 1 + len (reverse as) := by rw [ih]
+      _ = len (reverse (cons a as)) := by
+        rw [reverse]
+        sorry -- would need auxiliary lemma about reverse.loop
+        )
+
+theorem reverse_reverse {α : Type u} (as : List α)
+  : as = reverse (reverse as) := by
+  have loopstarter (as : List α)
+    : as = reverse.loop empty as := rfl
+  have rrloop (as ras : List α)
+    : reverse.loop as ras = reverse (reverse.loop ras as) :=
+    List.recOn as
+    (List.recOn ras (by simp [reverse.loop, reverse]) (by
+      intros a as1 ih
+      admit
+    ))
+    (by admit)
+  calc as
+    _ = reverse.loop empty as := loopstarter as
+    _ = reverse (reverse.loop as empty) := rrloop empty as
+    _ = reverse (reverse as) := by
+      rw [rrloop as empty, ← loopstarter as]
+
+theorem reverse_reverse' {α : Type u} (as : List α)
+  : as = reverse (reverse as) := by
+  have loopstarter (as : List α)
+    : reverse.loop empty as = as := rfl
+  have rrloop (as : List α)
+    : reverse (reverse.loop as empty) = as :=
+    List.recOn as
+    (by simp [reverse.loop, reverse])
+    (by
+      intros a as h1
+      rw [reverse.loop]
+      admit
+    )
+  calc as
+    _ = reverse (reverse.loop as empty) := by simp [rrloop]
+    _ = reverse (reverse as) := by rw [← reverse]
+
+
+variable (C : Nat → Type u)
+variable (α : Type)
+variable (r : Prop)
+
+#check List.below
+#reduce List.below (α := Nat) (motive := fun l => len l = len l) (cons 3 empty)
